WIP making tactics and lemmas for working with maps modular, not just for variables

src/Base.v
@@ -1,4 +1,6 @@
-From Stdlib Require FSets.FMapList FSets.FSetList FSets.FMapFacts
+From Stdlib Require FSets.FMapList FSets.FSetList 
+                            FSets.FMapFacts
+                            FSets.FMapInterface
                             OrderedType OrderedTypeEx.
 From QuantumLib Require Import Matrix Pad Quantum.
 From Stdlib Require Import String Morphisms (* for Proper *).
@@ -10,45 +12,790 @@ Open Scope list_scope.
 Declare Scope qoreo.
 Create HintDb var_db.
 
+(** Generic map theory: extends FMapFacts.Properties with definitions and
+    theorems about [Singleton], [concat], and associated tactics. The module
+    is parameterized over an arbitrary [FMapInterface.S] so it can be
+    instantiated for any key type. *)
+Module FMap_fun (E : OrderedType.OrderedType) (M : FMapInterface.Sfun E) (FSet : FSetInterface.Sfun E).
+  Import M.
+  (* type t = M.t, type key = M.key = V0.t *)
+  Module Export Properties := FMapFacts.WProperties_fun E M. (* Includes module F *)
+  Module FSetProperties := FSetFacts.WFacts_fun E FSet.
+
+  Definition Singleton {A} (x : key) (a : A) (m : M.t A) : Prop :=
+    M.Equal m (M.add x a (M.empty _)).
+
+  Definition concat {A} (m1 m2 : t A) : t A :=
+    M.fold (fun k v acc => M.add k v acc) m1 m2.
+
+  Definition domain {A} (m : M.t A) : FSet.t :=
+      let f := fun x _ s => FSet.add x s in
+      M.fold f m FSet.empty.
+  Definition Partition {A} := @Properties.Partition A.
+
+  (* Rewrite/auto databases *)
+  #[global] Existing Instance F.EqualSetoid.
+  #[global] Hint Rewrite F.add_mapsto_iff : var_db.
+  #[global] Hint Rewrite F.empty_mapsto_iff : var_db.
+  #[global] Hint Rewrite F.add_in_iff : var_db.
+  #[global] Hint Rewrite F.map_o : var_db.
+  #[global] Hint Rewrite F.remove_o : var_db.
+  #[global] Hint Rewrite F.add_o : var_db.
+  #[global] Hint Rewrite F.empty_o : var_db.
+  #[global] Hint Rewrite F.map_in_iff : var_db.
+  #[global] Hint Resolve M.empty_1 : var_db.
+  #[global] Hint Resolve Properties.Partition_sym : var_db.
+
+  Module Proofs.
+
+  #[global] Instance singletonProper : forall A,
+    Proper (E.eq ==> @eq A ==> @M.Equal A ==> iff) (@Singleton A).
+  Proof.
+    intros A x1 x2 Heq a1 a2 Ha m1 m2 Hm. subst.
+    unfold Singleton.
+    rewrite Heq. rewrite Hm. reflexivity.
+  Qed.
+
+  (** Concatenation *)
+
+  Lemma concat_find : forall A (m1 m2 : M.t A) k,
+    M.find k (concat m1 m2) =
+    match M.find k m1 with
+    | Some v => Some v
+    | None => M.find k m2
+    end.
+  Proof.
+    intros.
+    unfold concat.
+    apply fold_rec; intros.
+    - replace (M.find k m) with (@None A); auto.
+      {
+        symmetry. apply F.not_find_in_iff.
+        intros [v Hin]. apply (H k v); auto.
+      }
+    - rewrite F.add_o.
+      unfold Add in H1.
+      rewrite H1.
+      rewrite F.add_o.
+      rewrite H2.
+      destruct (E.eq_dec k0 k); auto.
+  Qed.
+  #[global] Hint Rewrite concat_find : var_db.
+
+  #[global] Instance concatProper : forall A,
+    Proper (@M.Equal A ==> @M.Equal A ==> @M.Equal A) (@concat A).
+  Proof.
+    intros A m1 m2 Hm n1 n2 Hn.
+    intros z.
+    repeat rewrite concat_find.
+    rewrite Hm.
+    destruct (M.find z m2); auto.
+  Qed.
+
+  Lemma concat_in : forall A x (m1 m2 : M.t A),
+    M.In x (concat m1 m2) <-> M.In x m1 \/ M.In x m2.
+  Proof.
+    intros A x m1 m2.
+    repeat rewrite F.in_find_iff.
+    rewrite concat_find.
+    destruct (M.find x m1); auto.
+    * split; [intros | intros [? | ?]]; auto.
+      inversion 1.
+    * split; [intros | intros [? | ?]]; auto.
+  Qed.
+  #[global] Hint Rewrite concat_in : var_db.
+
+  Lemma map_concat : forall {A B} (f : A -> B) m1 m2,
+    M.Equal (M.map f (concat m1 m2))
+            (concat (M.map f m1) (M.map f m2)).
+  Proof.
+      intros.
+      intros z.
+      autorewrite with var_db.
+      destruct (M.find z m1); auto.
+  Qed.
+  #[global] Hint Rewrite @map_concat : var_db.
+
+  Lemma concat_assoc : forall {A} (m1 m2 m3 : M.t A),
+    M.Equal (concat m1 (concat m2 m3)) (concat (concat m1 m2) m3).
+  Proof.
+      intros.
+      intros z.
+      autorewrite with var_db.
+      destruct (M.find z m1); auto.
+  Qed.
+
+  Lemma domain_add_iff : forall A x z (a : A) m0 m,
+    Add x a m0 m ->
+    FSet.In z (domain m) <-> (x = z) \/ FSet.In z (domain m0).
+  Admitted.
+
+  Lemma domain_remove : forall A x m,
+    FSet.Equal (domain (remove x m)) (FSet.remove x (@domain A m)).
+  Admitted.
+
+  (** Domain *)
+  #[global] Existing Instance FSetProperties.Equal_ST.
+  #[global] Instance domainProper : forall A,
+    Proper (@M.Equal A ==> @FSet.Equal) (@domain A).
+  Proof.
+    intros A m1 m2 Heq.
+    unfold domain.
+    apply fold_Equal; auto.
+    * apply FSetProperties.Equal_ST.
+    * intros x1 x2 Hx a1 a2 Ha X1 X2 HX; subst.
+      rewrite Hx. rewrite HX. reflexivity.
+    * intros x1 x2 ? ? ? Hneq z.
+      repeat rewrite FSetProperties.add_iff.
+      tauto.
+  Qed.
+      
+
+
+  (** Lemma about FSets *)
+
+  Lemma fset_in_union : forall x X1 X2,
+    FSet.In x (FSet.union X1 X2)
+    <->
+    FSet.In x X1 \/ FSet.In x X2.
+  Proof.
+    intros x X1 X2. split.
+    - apply FSet.union_1.
+    - intros [H | H].
+      + apply FSet.union_2; exact H.
+      + apply FSet.union_3; exact H.
+  Qed.
+  #[global] Hint Rewrite fset_in_union : var_db.
+
+  (** General properties of maps *)
+
+  Lemma remove_not_in : forall A x (m : M.t A),
+    ~ M.In x m ->
+    M.Equal
+      (M.remove x m)
+      m.
+  Proof.
+    intros ? ? ? Hin.
+    intros z.
+    autorewrite with var_db.
+    destruct (F.eq_dec x z) as [Heq | ?]; auto.
+    {
+      subst.
+      rewrite <- Heq.
+      apply F.not_find_in_iff in Hin.
+      auto.
+    }
+  Qed.
+
+  Lemma remove_map : forall A B x (f : A -> B) m,
+    M.Equal
+      (M.remove x (M.map f m))
+      (M.map f (M.remove x m)).
+  Proof.
+    intros A B x f m z;
+      autorewrite with var_db.
+    destruct (E.eq_dec x z) as [Heq | Hneq];
+      subst; simpl; auto.
+  Qed.
+  #[global] Hint Rewrite remove_map : var_db.
+
+  Ltac compare x y :=
+    let Heq := fresh "Heq" in
+    destruct (E.eq_dec x y) as [Heq | Heq];
+      try (rewrite <- Heq in *; clear Heq);
+      try contradiction;
+      try match goal with
+      | [ H : ~ E.eq ?x ?x |- _ ] => contradict H; reflexivity
+      end.
+
+  Ltac reduce_eq_dec :=
+    match goal with
+    | [ |- context[E.eq_dec ?x ?y] ] => compare x y
+    | [ H : context[E.eq_dec ?x ?y] |- _ ] => compare x y
+    end.
+
+  Lemma remove_add : forall A x y (v : A) Gamma,
+    M.Equal
+      (M.remove x (M.add y v Gamma))
+      (if E.eq_dec x y then M.remove x Gamma else M.add y v (M.remove x Gamma)).
+  Proof.
+    intros.
+    intros z.
+    autorewrite with var_db.
+    repeat (reduce_eq_dec; autorewrite with var_db; auto).
+  Qed.
+  #[global] Hint Rewrite remove_add : var_db.
+
+  Lemma remove_empty : forall A x,
+    M.Equal (M.remove x (@M.empty A))
+      (@M.empty A).
+  Proof.
+    intros A x y.
+    autorewrite with var_db.
+    reduce_eq_dec; auto.
+  Qed.
+  #[global] Hint Rewrite remove_empty : var_db.
+
+  Lemma map_add : forall {A B} (f : A -> B) x a m,
+    M.Equal (M.map f (M.add x a m))
+            (M.add x (f a) (M.map f m)).
+  Proof.
+    intros.
+    intros z. autorewrite with var_db.
+    compare x z; auto.
+  Qed.
+  #[global] Hint Rewrite @map_add : var_db.
+
+  (** Empty maps *)
+
+  Lemma empty_map_equal : forall {A} (m : M.t A),
+    M.Empty m -> M.Equal m (M.empty A).
+  Proof.
+    intros A m Hempty k.
+    autorewrite with var_db.
+    destruct (M.find k m) eqn:Hfind; auto.
+    apply M.find_2 in Hfind. exfalso. eapply Hempty; eauto.
+  Qed.
+  #[global] Hint Resolve @empty_map_equal : var_db.
+
+  Lemma empty_map_Empty : forall {A B} (f : A -> B) m,
+    M.Empty (M.map f m) <->
+    M.Empty m.
+  Proof.
+    intros A B f m. 
+    split.
+    - intros Hempty k v Hmaps.
+      apply (Hempty k (f v)).
+      apply M.map_1; exact Hmaps.
+    - intros Hempty k v Hmaps.
+      apply F.map_mapsto_iff in Hmaps.
+      destruct Hmaps as [a [_ Ha]].
+      exact (Hempty k a Ha).
+  Qed.
+
+  Lemma empty_map_empty : forall {A B} (f : A -> B),
+    M.Equal (M.map f (M.empty A)) (M.empty B).
+  Proof.
+    intros A B f k.
+    autorewrite with var_db.
+    reflexivity.
+  Qed.
+  #[global] Hint Rewrite @empty_map_empty : var_db.
+
+  Lemma singleton_singleton : forall A x (a : A),
+    Singleton x a (M.add x a (M.empty _)).
+  Proof.
+    intros A x a.
+    intros z.
+    reflexivity.
+  Qed.
+
+  Lemma singleton_remove : forall {A} (a : A) x m,
+    Singleton x a m ->
+    M.Empty (M.remove x m).
+  Proof.
+    intros A a x m H.
+    unfold Singleton in H.
+    rewrite H.
+    autorewrite with var_db.
+    compare x x.
+    autorewrite with var_db.
+    apply M.empty_1.
+  Qed.
+  #[global] Hint Resolve @singleton_remove : var_db.
+
+  Ltac subst_eq_hypothesis_fwd m :=
+    repeat match goal with
+    | [ Heq : M.Equal m _, H : context[m] |- _ ] =>
+      setoid_rewrite Heq in H
+    | [ Heq : M.Equal m _ |- context[m] ] =>
+      setoid_rewrite Heq
+    end;
+    (* if there are no more occurrences of m, clear Heq *)
+    try match goal with
+    | [ Heq : M.Equal m _ |- _ ] => clear m Heq
+    end.
+
+  Ltac subst_eq_hypothesis_bwd m :=
+    repeat match goal with
+    | [ Heq : M.Equal _ m, H : context[m] |- _ ] =>
+      setoid_rewrite <- Heq in H
+    | [ Heq : M.Equal _ m |- context[m] ] =>
+      setoid_rewrite <- Heq
+    end.
+    (* if there are no more occurrences of m, clear Heq *)
+    (*
+    try match goal with
+    | [ Heq : M.Equal _ m |- _ ] => clear m Heq
+    end.
+    *)
+
+  Ltac subst_map :=
+    repeat match goal with
+    | [ Heq : M.Equal ?m ?m |- _ ] => clear Heq; try clear m
+    | [ m : M.t _ |- _ ] =>
+      match goal with
+      | [ Heq : M.Equal m _ |- _ ] =>
+        subst_eq_hypothesis_fwd m;
+        try clear m Heq
+      | [ Heq : M.Equal _ m |- _ ] =>
+        subst_eq_hypothesis_bwd m;
+        try clear m Heq
+      end
+    end.
+
+  Ltac simpl_Empty :=
+      match goal with
+      | [ H : M.Empty (M.map _ _) |- _ ] =>
+        apply empty_map_Empty in H
+      | [ |- M.Empty (M.map _ _) ] =>
+        apply empty_map_Empty
+
+      (* Replace any instances of Empty m with m == empty
+      and substitute *)
+      | [ H : M.Empty ?m |- _ ] =>
+        apply empty_map_equal in H;
+        subst_map
+      end.
+
+  (** Lemmas about disjointness *)
+
+  Lemma concat_disjoint : forall {A} (m1 m2 m3 : M.t A),
+    Disjoint m1 (concat m2 m3) <->
+    Disjoint m1 m2 /\ Disjoint m1 m3.
+  Proof.
+    intros A m1 m2 m3.
+    unfold Disjoint.
+    repeat split; intros.
+    * specialize (H k); autorewrite with var_db in H.
+      firstorder.
+    * specialize (H k); autorewrite with var_db in H.
+      firstorder.
+    * autorewrite with var_db.
+      firstorder.
+  Qed.
+  #[global] Hint Rewrite @concat_disjoint : var_db.
+
+  Lemma disjoint_sym : forall {A} (m1 m2 : M.t A),
+    Disjoint m1 m2 ->
+    Disjoint m2 m1.
+  Proof.
+    intros ? ? ? H.
+    unfold Disjoint.
+    intros k; specialize (H k). firstorder.
+  Qed.
+
+  Lemma disjoint_map : forall {A B} (f : A -> B) m1 m2,
+    Disjoint (M.map f m1) (M.map f m2)
+    <-> Disjoint m1 m2.
+  Proof.
+    intros A B f m1 m2.
+    unfold Disjoint.
+    split; intros H k [Hin1 Hin2].
+    - apply (H k). split.
+      + apply F.map_in_iff; exact Hin1.
+      + apply F.map_in_iff; exact Hin2.
+    - apply F.map_in_iff in Hin1.
+      apply F.map_in_iff in Hin2.
+      exact (H k (conj Hin1 Hin2)).
+  Qed.
+
+  Lemma disjoint_empty_1 : forall A m,
+    Disjoint (M.empty A) m.
+  Proof.
+    intros. intros z.
+    rewrite F.empty_in_iff.
+    intros [? ?]; contradiction.
+  Qed.
+
+  Lemma disjoint_empty_2 : forall A m,
+    Disjoint m (M.empty A).
+  Proof.
+    intros. intros z.
+    rewrite F.empty_in_iff.
+    intros [? ?]; contradiction.
+  Qed.
+  #[global] Hint Resolve disjoint_empty_1 disjoint_empty_2 : var_db.
+
+  Lemma disjoint_remove_1 : forall {A} (m1 m2 : M.t A) x,
+    Disjoint m1 m2 ->
+    Disjoint (M.remove x m1) m2.
+  Admitted.
+
+  Lemma disjoint_remove_2 : forall {A} (m1 m2 : M.t A) x,
+    Disjoint m1 m2 ->
+    Disjoint m1 (M.remove x m2).
+  Proof.
+    intros.
+    apply disjoint_sym. apply disjoint_remove_1.
+    apply disjoint_sym. auto.
+  Qed.
+
+  Ltac reduce_disjoint :=
+  repeat match goal with
+        | [ H : Disjoint ?m1 ?m2 |- Disjoint ?m2 ?m1 ] =>
+          apply disjoint_sym; exact H
+
+        | [ |- Disjoint (M.map _ _) (M.map _ _)] =>
+          apply disjoint_map
+        | [ H : Disjoint (M.map _ _) (M.map _ _) |- _] =>
+          apply disjoint_map in H
+
+        | [ |- Disjoint _ (concat _ _)] =>
+          apply concat_disjoint; split
+        | [ |- Disjoint _ (concat _ _)] =>
+          apply disjoint_sym; apply concat_disjoint; split; apply disjoint_sym
+        | [ H : Disjoint _ (concat _ _) |- _ ] =>
+          apply concat_disjoint in H;
+          destruct H
+        | [ H : Disjoint (concat _ _) _ |- _ ] =>
+          apply disjoint_sym in H;
+          apply concat_disjoint in H;
+          let H1 := fresh "Hdisj" in
+          let H2 := fresh "Hdisj" in
+          destruct H as [H1 H2];
+          apply disjoint_sym in H1;
+          apply disjoint_sym in H2
+
+        | [ |- Disjoint (M.empty _) _ ] =>
+          apply disjoint_empty_1
+        | [ |- Disjoint _ (M.empty _) ] =>
+          apply disjoint_empty_2
+  end.
+
+  (** Reflection between partition and concat *)
+
+  Lemma partition_concat : forall {A} (m m1 m2 : M.t A),
+    Partition m m1 m2 <->
+    Disjoint m1 m2 /\ M.Equal m (concat m1 m2).
+  Proof.
+    intros A m m1 m2.
+    split; [intros [Hdisj Hpart] | intros [Hdisjoint Heq]].
+    * split; auto.
+      intros k.
+      rewrite concat_find.
+      destruct (M.find k m1) as [ a |] eqn:Hfind1.
+      { specialize (Hpart k a);
+        repeat rewrite F.find_mapsto_iff in Hpart.
+        apply Hpart; auto.
+      }
+      destruct (M.find k m2) as [a | ] eqn:Hfind2.
+      {
+        specialize (Hpart k a);
+        repeat rewrite F.find_mapsto_iff in Hpart.
+        apply Hpart; auto.
+      }
+      destruct (M.find k m) as [a | ] eqn:Hfind; auto.
+      { (* contradiction *)
+        contradict Hfind.
+        specialize (Hpart k a);
+        repeat rewrite F.find_mapsto_iff in Hpart.
+        rewrite Hpart, Hfind1, Hfind2.
+        inversion 1; discriminate.
+      }
+    * split; auto.
+      intros k a.
+      rewrite Heq.
+      repeat rewrite F.find_mapsto_iff.
+      rewrite concat_find.
+      destruct (M.find k m1) eqn:Hfind1.
+      {
+        destruct (M.find k m2) eqn:Hfind2; auto;
+          try (firstorder; fail).
+        { unfold Disjoint in Hdisjoint.
+          exfalso; apply (Hdisjoint k).
+          repeat rewrite F.in_find_iff.
+          rewrite Hfind1, Hfind2.
+          split; inversion 1.
+        }
+        firstorder. discriminate.
+      }
+      destruct (M.find k m2) eqn:Hfind2; auto.
+      {
+        firstorder; try discriminate.
+      }
+      firstorder.
+  Qed.
+
+  Lemma concat_sym : forall {A} (m1 m2 : M.t A),
+    Disjoint m1 m2 ->
+    M.Equal (concat m1 m2) (concat m2 m1).
+  Proof.
+    intros A m1 m2 Hdisj z.
+    autorewrite with var_db.
+    destruct (M.find z m1) eqn:Hfind1; destruct (M.find z m2) eqn:Hfind2; auto.
+    exfalso. apply (Hdisj z). split.
+    - apply F.in_find_iff. rewrite Hfind1; discriminate.
+    - apply F.in_find_iff. rewrite Hfind2; discriminate.
+  Qed.
+
+  Ltac reflect_partition :=
+    repeat match goal with
+          | [ H : Partition ?m ?m1 ?m2 |- _ ] =>
+            apply partition_concat in H;
+            let Hdisj := fresh "Hdisj" in
+            let Heq := fresh "Heq" in
+            destruct H as [Hdisj Heq];
+            subst_map
+          | [ |- Partition ?m ?m1 ?m2 ] =>
+            apply partition_concat; split
+          | [ H : context[M.map _ (concat _ _)] |- _] =>
+            rewrite map_concat in H
+          | [ |- context[M.map _ (concat _ _)] ] =>
+            rewrite map_concat
+    end.
+
+  (** Lemmas about Partition *)
+
+  (*** If Δ(x0)=τ0 and Δ==Δ1,Δ2 and x ∉ Δ2 then Δ1(x0)=τ0 *)
+  Lemma partition_not_in_r : forall {A} Δ Δ2 Δ1 x (τ : A),
+    M.MapsTo x τ Δ ->
+    Partition Δ Δ1 Δ2 ->
+    ~ (M.In x Δ2) ->
+    M.MapsTo x τ Δ1.
+  Proof.
+    intros ? ? ? ? x τ Hx [Hdisjoint Hmapsto] Hnotin.
+    apply Hmapsto in Hx.
+    destruct Hx; auto.
+    * contradict Hnotin.
+      exists τ; auto.
+  Qed.
+
+  Lemma partition_empty_l : forall A m,
+    Partition m (M.empty A) m.
+  Proof.
+    intros.
+    reflect_partition.
+    * reduce_disjoint.
+    * intros z. autorewrite with var_db; auto.
+  Qed.
+  #[global] Hint Resolve partition_empty_l : var_db.
+
+  Lemma partition_empty_r : forall A m,
+    Partition m m (M.empty A).
+  Proof.
+    intros.
+    reflect_partition.
+    * reduce_disjoint.
+    * intros z. autorewrite with var_db; auto.
+      destruct (M.find z m); auto.
+  Qed.
+  #[global] Hint Resolve partition_empty_r : var_db.
+
+  Lemma partition_add_l : forall A x (a:A) m m1 m2,
+    Partition m m1 m2 ->
+    ~ M.In x m2 ->
+    Partition (M.add x a m) (M.add x a m1) m2.
+  Proof.
+    intros.
+    reflect_partition.
+    * unfold Disjoint in *.
+      intros k [Hin1 Hin2].
+      autorewrite with var_db in Hin1.
+      apply (Hdisj k). split; auto.
+      destruct Hin1 as [Heq | ?]; auto.
+      rewrite Heq in *; clear Heq.
+      contradiction.
+    * intros z. autorewrite with var_db.
+      reduce_eq_dec; auto.
+  Qed.
+
+  Lemma partition_add_r : forall A x (a:A) m m1 m2,
+    Partition m m1 m2 ->
+    ~ M.In x m1 ->
+    Partition (M.add x a m) m1 (M.add x a m2).
+  Proof.
+    intros.
+    apply Partition_sym.
+    apply partition_add_l; auto.
+    apply Partition_sym; auto.
+  Qed.
+
+  Lemma partition_remove : forall {A} x0 (Δ Δ1 Δ2 : M.t A),
+    Partition Δ Δ1 Δ2 ->
+    Partition (M.remove x0 Δ) (M.remove x0 Δ1) (M.remove x0 Δ2).
+  Proof.
+    intros A x0 Δ Δ1 Δ2 Hpart.
+    reflect_partition.
+    - (* Disjoint (remove x0 Δ1) (remove x0 Δ2) *)
+      apply disjoint_remove_1.
+      apply disjoint_remove_2.
+      auto.
+    -
+      intros k.
+      autorewrite with var_db in *.
+      reduce_eq_dec; auto.
+  Qed.
+
+  Lemma partition_empty_inv1 : forall {A} (Δ1 Δ2 : M.t A),
+    Partition (M.empty _) Δ1 Δ2 ->
+    M.Equal Δ1 (M.empty _).
+  Admitted.
+
+  Lemma partition_empty_inv2 : forall {A} (Δ1 Δ2 : M.t A),
+    Partition (M.empty _) Δ1 Δ2 ->
+    M.Equal Δ2 (M.empty _).
+  Admitted.
+
+  Lemma partition_map_iff : forall A B (f : A -> B) m m1 m2,
+    Partition m m1 m2 <->
+    Partition (M.map f m) (M.map f m1) (M.map f m2).
+  Admitted.
+
+  Lemma partition_map_inv : forall A B (f : A -> B) m n1 n2,
+    Partition (M.map f m) n1 n2 ->
+    exists m1 m2,
+      M.Equal n1 (M.map f m1)
+      /\
+      M.Equal n2 (M.map f m2)
+      /\
+      Partition m m1 m2.
+  Admitted.
+
+  Lemma partition_empty1_eq : forall A m m0,
+      Partition m (M.empty A) m0 ->
+      M.Equal m m0.
+  Admitted.
+
+  Lemma partition_empty2_eq : forall A m m0,
+      Partition m m0 (M.empty A) ->
+      M.Equal m m0.
+  Admitted.
+
+  Ltac reduce_partition :=
+    match goal with
+
+      (* Partitions with the empty map *)
+      | [ H : Partition (M.empty _) ?D1 ?D2 |- _ ] =>
+        let H1 := fresh "H1" in
+        let H2 := fresh "H2" in
+        assert (H1 : M.Equal D1 (M.empty _))
+          by (exact (partition_empty_inv1 D1 D2 H));
+        assert (H2 : M.Equal D2 (M.empty _))
+          by (exact (partition_empty_inv2 D1 D2 H));
+        subst_map;
+        try clear H
+
+      | [ H : Partition ?m (M.empty _) ?m0 |- _ ] =>
+        apply partition_empty1_eq in H;
+        subst_map
+      | [ H : Partition ?m ?m0 (M.empty _) |- _ ] =>
+        apply partition_empty2_eq in H;
+        subst_map
+
+      (* Partitions with remove *)
+      | [ |- Partition (M.remove ?x _) (M.remove ?x _) (M.remove ?x _) ] =>
+        apply partition_remove
+
+      (* Partitions with map *)
+      | [ |- Partition (M.map ?f _) (M.map ?f _) (M.map ?f _) ] =>
+        apply partition_map_iff
+      | [ H : Partition (M.map ?f _) (M.map ?f _) (M.map ?f _) |- _ ] =>
+        apply partition_map_iff in H
+
+      | [H : Partition (M.map ?f ?m) ?n1 ?n2 |- _] =>
+        let m1 := fresh "m1" in
+        let m2 := fresh "m2" in
+        let Heq1 := fresh "Heq1" in
+        let Heq2 := fresh "Heq2" in
+        destruct (partition_map_inv _ _ _ _ _ _ H)
+          as [m1 [m2 [Heq1 [Heq2 Hpart]]]]; auto;
+        subst_map; try rewrite Heq1, Heq2 in *; try clear n1 Heq1 n2 Heq2
+    end.
+
+  Ltac vsimpl :=
+  repeat match goal with
+  | [ |- M.Empty _ ] => simpl_Empty
+  | [ H : M.Empty _ |- _ ] => simpl_Empty
+
+  | [ |- Disjoint _ _ ] => reduce_disjoint
+  | [ H : Disjoint _ _ |- _ ] => reduce_disjoint
+
+  | [ |- context[Partition _ _ _ ]] =>
+    reduce_partition
+  | [ H : context[Partition _ _ _ ] |- _ ] =>
+    reduce_partition
+
+  | [ H : M.Equal _ _ |- _ ] => subst_map
+  end.
+  End Proofs.
+
+
+  Module Tactics.
+  (**
+    Provides:
+      * compare x y       - destructs Map.E.eq_dec x y and substitutes
+      * reduce_eq_dec     - applies compare to goals/hypotheses containing Map.E.eq_dec
+      * subst_map         - eliminates hypotheses of the form Map.Equal m1 m2 by rewriting
+      * reflect_partition - converts Partition hypotheses into Disjoint + Map.Equal (concat) form
+      * vsimpl            - simplifies hypotheses and goals that use maps
+
+    vsimpl builds on the following tactics in MapFacts:
+      * simpl_Empty       - simplifies Map.Empty goals/hypotheses and substitutes
+      * reduce_disjoint   - simplifies Disjoint goals/hypotheses using symmetry and concat lemmas
+      * reduce_partition  - simplifies Partition hypotheses
+
+    In addition, there are rewrite and auto databases for simplifying goals:
+      * autorewrite with var_db [in H]
+      * auto/eauto with var_db
+  *)
+    Ltac compare x y := Proofs.compare x y.
+    Ltac reduce_eq_dec := Proofs.reduce_eq_dec.
+    Ltac subst_map := Proofs.subst_map.
+    Ltac reflect_partition := Proofs.reflect_partition.
+    Ltac vsimpl := Proofs.vsimpl.
+  End Tactics.
+
+End FMap_fun.
+
+Module FMap (E0 : OrderedType.OrderedType) <: FMapInterface.S.
+  Module M := FSets.FMapList.Make E0.
+  Include M.
+    
+  Module S := FSets.FSetList.Make E.
+
+  Module MProofs := FMap_fun E M S.
+  Include MProofs.
+End FMap.
+
 Module Var.
 
   Module V := OrderedTypeEx.UOT_to_OT (OrderedTypeEx.Nat_as_OT).
-  Definition t := V.t.
-  Definition eq_dec : forall (x y : t), {x=y} + {x <> y} := eq_nat_dec.
-  
-  Module Map := FSets.FMapList.Make(V).
-  Module MapFacts := FMapFacts.Properties(Map).
-  Module FSet := FSets.FSetList.Make(V).
-
-  Definition domain {A} (m : Map.t A) : FSet.t :=
-    let f := fun x _ s => FSet.add x s in
-    Map.fold f m FSet.empty.
+  Include V.
+  Module Map := FMap V.
+  Module FSet := Map.S.
 
   Definition fresh {A} (m : Map.t A) :=
     let f := fun x _ z_fresh => if Nat.leb z_fresh x then (x+1)%nat else z_fresh in
     Map.fold f m 0%nat.
 
-  Definition Singleton {A} x a (m : Map.t A) : Prop :=
-    Map.Equal m (Map.add x a (Map.empty _)).
+
+  (** General properties of Var-specific eq_dec (nat equality) *)
+
+  (*
+  Lemma eq_dec_refl : forall x,
+    eq_dec x x = left (eq_refl x).
+  Proof.
+    intros.
+    induction x; simpl; auto.
+    rewrite IHx; auto.
+  Qed.
+  #[global] Hint Rewrite eq_dec_refl : var_db.
+*)
 
 
-  Definition concat {A} (m1 m2 : Map.t A) : Map.t A :=
-  Map.fold (fun k v acc => Map.add k v acc) m1 m2.
+End Var.
+(*
+#[global] Hint Rewrite MapFacts.F.add_mapsto_iff : var_db.
+#[global] Hint Rewrite MapFacts.F.empty_mapsto_iff : var_db.
+#[global] Hint Rewrite MapFacts.F.add_in_iff : var_db.
+#[global] Hint Rewrite MapFacts.F.map_o : var_db.
+#[global] Hint Rewrite MapFacts.F.remove_o : var_db.
+#[global] Hint Rewrite MapFacts.F.add_o : var_db.
+#[global] Hint Rewrite MapFacts.F.empty_o : var_db.
+#[global] Hint Rewrite Var.MapFacts.F.map_in_iff : var_db.
 
-Module Proofs.
-
-  (* Create a rewrite database of MapFacts *)
-  #[global] Existing Instance MapFacts.F.EqualSetoid.
-  #[global] Hint Rewrite MapFacts.F.add_mapsto_iff : var_db.
-  #[global] Hint Rewrite MapFacts.F.empty_mapsto_iff : var_db.
-  #[global] Hint Rewrite MapFacts.F.add_in_iff : var_db.
-  #[global] Hint Rewrite MapFacts.F.map_o : var_db.
-  #[global] Hint Rewrite MapFacts.F.remove_o : var_db.
-  #[global] Hint Rewrite MapFacts.F.add_o : var_db.
-  #[global] Hint Rewrite MapFacts.F.empty_o : var_db.
-  #[global] Hint Rewrite Var.MapFacts.F.map_in_iff : var_db.
-
-  #[global] Hint Resolve Var.Map.empty_1 : var_db.
+#[global] Hint Resolve Var.Map.empty_1 : var_db.
 
   #[global] Instance singletonProper : forall A,
     Proper (@eq t ==> @eq A ==> @Map.Equal A ==> iff) (@Singleton A).
@@ -767,6 +1514,7 @@ Module Tactics.
 End Tactics.
 
 End Var.
+*)
 
 
 Inductive unitary :=
@@ -890,7 +1638,7 @@ Module Config.
     let qs := List.map (fun x => find x refs) xs in
     apply_matrix cfg (gate_to_matrix _ U qs).
 
-    
+  (*
   Lemma test1 : gate_to_matrix 2 CNOT [0;1]%nat = cnot.
   Proof.
     assert (H : WF_Matrix (gate_to_matrix 2 CNOT [0%nat; 1%nat])).
@@ -911,12 +1659,14 @@ Module Config.
   Proof.
     simpl. unfold pad. simpl. Msimpl; auto.
   Qed.
+  *)
 
 End Config.
 
 (* This could be instantiated in different ways. *)
 
 Module Actor.
+
 
   Lemma bool_dec_refl : forall (b : bool), bool_dec b b = left (eq_refl b).
   Proof. destruct b; auto. Qed.
@@ -928,39 +1678,21 @@ Module Actor.
     reflexivity.
   Qed.
 
-  Module Export V := OrderedTypeEx.UOT_to_OT (OrderedTypeEx.String_as_OT).
-  Definition t := V.t.
-  Definition eq_dec : forall (x y : t), {x=y} + {x <> y} := string_dec.
 
-
-  Lemma eq_dec_refl : forall A, eq_dec A A = left (eq_refl A).
-  Proof.
-    induction A; auto.
-    simpl. rewrite IHA. simpl.
-    rewrite ascii_dec_refl.
-    reflexivity.
-  Qed.
+  Module V := OrderedTypeEx.UOT_to_OT (OrderedTypeEx.String_as_OT).
+  Include V.
   
-  Module Map := FSets.FMapList.Make(V).
-  Module MapFacts := FMapFacts.Properties(Map).
-  Module FSet := FSets.FSetList.Make(V).
-  Module FSetFacts := FSetFacts.WFacts(FSet).
+  Module Map := FMap(V).
+  Module FSet := Map.S.
 
-  #[global] Existing Instance MapFacts.F.EqualSetoid.
-
-  Definition domain {A} (m : Map.t A) : FSet.t :=
-    let f := fun x _ s => FSet.add x s in
-    Map.fold f m FSet.empty.
-
-  Definition Singleton {A} x a (m : Map.t A) : Prop :=
-    Map.Equal m (Map.add x a (Map.empty _)).
-
+(*  #[global] Existing Instance MapProofs.F.EqualSetoid.*)
 
   Create HintDb actor_db.
-  #[global] Hint Rewrite Actor.FSetFacts.inter_iff : actor_db.
+  (*
+  #[global] Hint Rewrite Actor.FSet.Facts.inter_iff : actor_db.
   #[global] Hint Rewrite Actor.FSetFacts.add_iff : actor_db.
   #[global] Hint Rewrite Actor.FSetFacts.singleton_iff : actor_db.
-
+*)
 
 End Actor.
 
